begin on support for infinite signatures

lib/common.ml
@@ -308,7 +308,7 @@ let print_fun (f: Poulet4.P4flatToGCL.p4funs) : string =
   | BFalse -> "false"
   | BBitLit (width, value) ->
     Bigint.to_string value
-  | BTable (name, _) ->
+  | BTable name ->
     "table_symb__" ^ name
   | BProj1 -> "first"
   | BProj2 -> "second"
@@ -318,6 +318,16 @@ let print_fun (f: Poulet4.P4flatToGCL.p4funs) : string =
 let print_rel r : string =
   failwith "no relation symbols..."
 
+let print_ident (printer: 'a -> string) (i: 'a Poulet4.Sig.ident) : string =
+  let open Poulet4.Sig in
+  match i with
+  | SSimple n -> printer n
+  | SIdx (n, args) ->
+    Printf.sprintf "(_ %s %s)"
+      (printer n)
+      (List.map ~f:string_of_int args
+       |> String.concat ~sep:" ")
+
 let rec print_tm vp tm : string =
   let open Poulet4.Spec in
   match tm with
@@ -325,9 +335,9 @@ let rec print_tm vp tm : string =
   | TFun (f, args) ->
     if List.length args > 0
     then Printf.sprintf "(%s %s)"
-        (print_fun f)
+        (print_ident print_fun f)
         (print_tms vp args)
-    else print_fun (Obj.magic f)
+    else print_ident print_fun f
 
 and print_tms vp tms : string =
   List.map ~f:(print_tm vp) tms
@@ -361,9 +371,9 @@ let check_refinement ((prog_l, prog_r), rel) =
     Poulet4.GGCL.Dijkstra.seq_prod_wp
       String.equal
       String.equal in
-  match Poulet4.P4flatToGCL.prog_to_stmt prog_l,
-        Poulet4.P4flatToGCL.prog_to_stmt prog_r with
-  | Ok prog_l_gcl, Ok prog_r_gcl ->
+  match Poulet4.P4flatToGCL.prog_to_stmt prog_l Poulet4.P4flatToGCL.initial_p4sig,
+        Poulet4.P4flatToGCL.prog_to_stmt prog_r Poulet4.P4flatToGCL.initial_p4sig with
+  | Ok (prog_l_gcl, _), Ok (prog_r_gcl, _) ->
     let vc = wp prog_l_gcl prog_r_gcl rel in
     Printf.printf "\n%s\n\n" (print_fm sum_printer vc);
   | _, _ ->
