coq/lib/P4flat/P4flatToGCL.v
@@ -3,6 +3,7 @@ Require Import Coq.NArith.NArith.
 Require Import Poulet4.P4flat.Syntax.
 Require Import Poulet4.P4flat.GGCL.
 Require Import Poulet4.Monads.Result.
+Require Import Poulet4.Monads.State.
 Import ResultNotations.
 Import Dijkstra.
 
@@ -15,26 +16,45 @@ Inductive p4sorts :=
 | Bit (width: N)
 | Prod (s1 s2 : p4sorts)
 | ActionName.
+Scheme Equality for p4sorts.
+Instance p4sorts_EqDec : EqDec p4sorts eq := 
+  p4sorts_eq_dec.
 
 Inductive p4funs :=
 | BTrue
 | BFalse
 | BBitLit (width: N) (val: Z)
 | BTable (name: string)
-         (key: p4sorts)
-         (* no action data for now *)
 | BProj1
 | BProj2
 (* Better for this to be an enum or at least an integer *)
 | BAction (name: string).
-
+Scheme Equality for p4funs.
+Instance p4funs_EqDec : EqDec p4funs eq := 
+  p4funs_eq_dec.
 
 Inductive p4rels :=
 (* no relation symbols *)
 .
+Scheme Equality for p4rels.
+Instance p4rels_EqDec : EqDec p4rels eq := 
+  p4rels_eq_dec.
+
+Definition p4sig :=
+  Sig.signature p4sorts p4funs p4rels.
+
+Definition initial_p4sig : p4sig :=
+  {| Sig.sig_sorts := [ (Bool, 0); (ActionName, 0) ];
+    Sig.sig_funs := fun f =>
+                        if f == Sig.SSimple BTrue
+                        then Some ([], (Sig.SSimple Bool))
+                        else if f == Sig.SSimple BFalse
+                             then Some ([], (Sig.SSimple Bool))
+                             else None;
+     Sig.sig_rels := fun _ => None |}.
 
 Definition mk_action (name: string) : Spec.tm var p4funs :=
-  Spec.TFun (BAction name) [].
+  Spec.TFun (Sig.SSimple (BAction name)) [].
 
 Definition lhs_to_var (e: Expr.e) : result string var :=
   match e with
@@ -44,65 +64,67 @@ Definition lhs_to_var (e: Expr.e) : result string var :=
 
 Definition e_to_tm (e: Expr.e) : result string (Spec.tm var p4funs) :=
   match e with
-  | Expr.Bit width val => ok (Spec.TFun (BBitLit width val) [])
+  | Expr.Bit width val => ok (Spec.TFun (Sig.SSimple (BBitLit width val)) [])
   | Expr.Var _ name _ => ok (Spec.TVar name)
   | _ => error "e_to_tm unimplemented"
   end.
 
-Fixpoint s_to_stmt (s: Stmt.s) : result string (stmt var p4funs p4rels) :=
+Fixpoint s_to_stmt (s: Stmt.s) : StateT p4sig (result string) (stmt var p4funs p4rels) :=
   match s with
-  | Stmt.Skip => ok (GSkip _ _ _)
-  | Stmt.Return e => error "return unimplemented"
-  | Stmt.Exit => error "exit unimplemented"
+  | Stmt.Skip => mret (GSkip _ _ _)
+  | Stmt.Return e => state_lift (error "return unimplemented")
+  | Stmt.Exit => state_lift (error "exit unimplemented")
   | Stmt.Assign lhs rhs =>
-      let* lhs' := lhs_to_var lhs in
-      let* rhs' := e_to_tm rhs in
-      ok (GAssign lhs' rhs')
+      let* lhs' := state_lift (lhs_to_var lhs) in
+      let* rhs' := state_lift (e_to_tm rhs) in
+      mret (GAssign lhs' rhs')
   | Stmt.ExternCall extern_instance_name method_name type_args args returns =>
-      error "extern call unimplemented"
+      state_lift (error "extern call unimplemented")
   | Stmt.Table ctrl_plane_name key actions =>
-      let* key' := sequence (List.map e_to_tm key) in
+      let* key' := state_lift (sequence (List.map e_to_tm key)) in
       (* XXX generate an actually fresh variable here *)
       let result_var := ctrl_plane_name ++ "__res" in
-      let call_tm := Spec.TFun (BTable ctrl_plane_name (Bit 8%N)) key' in
+      let call_tm := Spec.TFun (Sig.SSimple (BTable ctrl_plane_name)) key' in
       let call_stmt := GAssign result_var call_tm in
-      let act_choice := Spec.TFun BProj1 [Spec.TVar result_var] in
+      let act_choice := Spec.TFun (Sig.SSimple BProj1) [Spec.TVar result_var] in
       let* actions_stmts :=
-        sequence (List.map (fun '(name, stmt) =>
-                              let+ stmt' := s_to_stmt stmt in  
-                              GSeq (GAssume (Spec.FEq act_choice (mk_action name)))
-                                   stmt')
+        sequence (List.map (fun '(name, params, stmt) =>
+                              let* stmt' := s_to_stmt stmt in  
+                              mret (GSeq (GAssume (Spec.FEq act_choice (mk_action name)))
+                                         stmt'))
                            actions) in
       let actions_stmt := List.fold_right GChoice (GSkip _ _ _) actions_stmts in
-      ok (GSeq call_stmt actions_stmt)
+      mret (GSeq call_stmt actions_stmt)
   | Stmt.Var original_name (inl typ) tail =>
       (* declaration is a no-op. *)
       s_to_stmt tail
   | Stmt.Var original_name (inr rhs) tail =>
-      let* rhs' := e_to_tm rhs in
+      let* rhs' := state_lift (e_to_tm rhs) in
       let* tail' := s_to_stmt tail in
-      ok (GSeq (GAssign original_name rhs') tail')
+      mret (GSeq (GAssign original_name rhs') tail')
   | Stmt.Seq head tail =>
       let* head' := s_to_stmt head in
       let* tail' := s_to_stmt tail in
-      ok (GSeq head' tail')
+      mret (GSeq head' tail')
   | Stmt.Conditional guard tru_blk fls_blk =>
-      let* guard' := e_to_tm guard in
-      let then_cond := Spec.FEq guard' (Spec.TFun BTrue []) in
+      let* guard' := state_lift (e_to_tm guard) in
+      let then_cond := Spec.FEq guard' (Spec.TFun (Sig.SSimple BTrue) []) in
       let else_cond := Spec.FNeg then_cond in
       let* tru_blk' := s_to_stmt tru_blk in
       let* fls_blk' := s_to_stmt fls_blk in
-      ok (GChoice (GSeq (GAssume then_cond) tru_blk')
-                  (GSeq (GAssume else_cond) fls_blk'))
+      mret (GChoice (GSeq (GAssume then_cond) tru_blk')
+                    (GSeq (GAssume else_cond) fls_blk'))
   end.
 
-Definition prog_to_stmt (p: TopDecl.prog) :=
-  let* (_, main_args) := TopDecl.find_decl "main" p
-                         >>= TopDecl.expect_pkg in
+Definition prog_to_stmt (p: TopDecl.prog) : StateT p4sig
+                                                   (result string)
+                                                   (stmt var p4funs p4rels) :=
+  let* (_, main_args) := state_lift (TopDecl.find_decl "main" p
+                                     >>= TopDecl.expect_pkg) in
   let* ctrl := match main_args with
-               | [ctrl] => ok ctrl
-               | _ => error "wrong number of args to main pkg (expected exactly 1)"
+               | [ctrl] => mret ctrl
+               | _ => state_lift (error "wrong number of args to main pkg (expected exactly 1)")
                end in
-  let* (_, cparams, cstmt) := TopDecl.find_decl ctrl p
-                              >>= TopDecl.expect_controlblock in
+  let* (_, cparams, cstmt) := state_lift (TopDecl.find_decl ctrl p
+                                          >>= TopDecl.expect_controlblock) in
   s_to_stmt cstmt.
