coq/lib/P4flat/Sig.v
@@ -14,32 +14,88 @@ Local Open Scope bool_scope.
 *)
 Definition vocab := Type.
 
+Section Ident.
+  Context (T: Type).
+  Context `{@EqDec T eq eq_equivalence}.
+
+  Inductive ident :=
+  | SSimple (base: T)
+  (* length of args should always be > 0 *)
+  | SIdx (base: T) (args: list nat).
+
+  #[global]
+  Instance ident_EqDec : EqDec ident eq.
+  Proof.
+    intros x y.
+    destruct x; destruct y.
+    - destruct (base == base0).
+      + left.
+        congruence.
+      + right.
+        congruence.
+    - right.
+      congruence.
+    - right.
+      congruence.
+    - destruct (base == base0).
+      + destruct (args == args0).
+        * left.
+          congruence.
+        * right.
+          congruence.
+      + right.
+        congruence.
+  Defined.
+End Ident.
+Arguments SSimple {T}.
+Arguments SIdx {T}.
+
 Section Signature.
-  Variables (sort_sym fun_sym rel_sym: vocab).
+  Variables (sort_sym func_sym rel_sym: vocab).
   Context `{sort_eq_dec: @EqDec sort_sym eq eq_equivalence}.
-  Context `{@EqDec fun_sym eq eq_equivalence}.
+  Context `{@EqDec func_sym eq eq_equivalence}.
   Context `{@EqDec rel_sym eq eq_equivalence}.
+
+  Definition sort := ident sort_sym.
+  Definition func := ident func_sym.
+  Definition rel := ident rel_sym.
+
+  Definition rank :=
+    list sort.
 
   (* Signature without arities *)
   Record signature : Type :=
-    { sig_sorts : list sort_sym;
-      sig_funs  : AList fun_sym (list sort_sym * sort_sym) eq;
-      sig_rels : AList rel_sym (list sort_sym) eq }.
+    { (* tracks arities for indexed sorts and is 0 if sort is simple *)
+      sig_sorts : AList sort_sym nat eq;
+      sig_funs  : func -> option (rank * sort);
+      sig_rels  : rel -> option rank }.
 
   Definition sig_get_sort (sig: signature) (s: sort_sym) :=
-    from_opt (List.find (fun s' => s ==b s') sig.(sig_sorts))
+    from_opt (AList.get sig.(sig_sorts) s)
              ("Sort symbol not found in sig.").
 
-  Definition sig_get_fun (sig: signature) (f: fun_sym) :=
-    from_opt (AList.get sig.(sig_funs) f)
+  Definition sig_get_fun (sig: signature) (f: func) :=
+    from_opt (sig.(sig_funs) f)
              ("Function symbol not found in sig.").
 
-  Definition sig_get_rel (sig: signature) (r: rel_sym) :=
-    from_opt (AList.get sig.(sig_rels) r)
-             ("Function symbol not found in sig.").
+  Definition sig_get_rel (sig: signature) (r: rel) :=
+    from_opt (sig.(sig_rels) r)
+             ("Relation symbol not found in sig.").
 
-  Definition sig_check_sort (sig: signature) (s: sort_sym) : bool :=
-    Result.is_okb (sig_get_sort sig s).
+  Definition sig_check_sort (sig: signature) (s: sort) : bool :=
+    match
+      match s with
+      | SSimple s =>
+          let* idx_arity := sig_get_sort sig s in
+          mret (idx_arity ==b 0)
+      | SIdx s args =>
+          let* idx_arity := sig_get_sort sig s in
+          mret (idx_arity ==b List.length args)
+      end
+    with 
+    | Ok b => b
+    | _ => false
+    end.
 
   (* Check that s is well-formed.
      This function should ensure that
@@ -47,23 +103,14 @@ Section Signature.
      - sig_funs and sig_rels have no duplicate keys
      - The arities in s use sorts drawn only from s.(sig_sorts) *)
   Definition check_signature (sig: signature) : bool :=
-    ListUtil.no_dups sort_eq_dec sig.(sig_sorts) &&
-    AList.key_unique sig.(sig_funs) &&
-    AList.key_unique sig.(sig_rels) &&
-    List.forallb (fun '(f, (arg_sorts, ret_sort)) =>
-                    List.forallb (sig_check_sort sig) arg_sorts
-                    && sig_check_sort sig ret_sort)
-                 sig.(sig_funs) &&
-    List.forallb (fun '(r, arg_sorts) =>
-                    List.forallb (sig_check_sort sig) arg_sorts)
-                 sig.(sig_rels).
+    AList.key_unique sig.(sig_sorts).
 End Signature.
 
-Arguments sig_sorts {sort_sym fun_sym rel_sym}.
-Arguments sig_funs {sort_sym fun_sym rel_sym}.
-Arguments sig_rels {sort_sym fun_sym rel_sym}.
-Arguments sig_get_sort {sort_sym fun_sym rel_sym _}.
-Arguments sig_check_sort {sort_sym fun_sym rel_sym _}.
-Arguments sig_get_fun {sort_sym fun_sym rel_sym _}.
-Arguments sig_get_rel {sort_sym fun_sym rel_sym _}.
-Arguments check_signature {sort_sym fun_sym rel_sym _ _ _}.
+Arguments sig_sorts {sort_sym func_sym rel_sym}.
+Arguments sig_funs {sort_sym func_sym rel_sym}.
+Arguments sig_rels {sort_sym func_sym rel_sym}.
+Arguments sig_get_sort {sort_sym func_sym rel_sym}.
+Arguments sig_check_sort {sort_sym func_sym rel_sym _}.
+Arguments sig_get_fun {sort_sym func_sym rel_sym}.
+Arguments sig_get_rel {sort_sym func_sym rel_sym}.
+Arguments check_signature {sort_sym func_sym rel_sym _}.
